Global types refactoring

theories/multiparty/invariant.v
@@ -187,9 +187,6 @@ Section pushpop.
     destruct l; sdec.
   Qed.
 
-  Definition bufs_empty {A} (bufs : bufsT participant participant A) :=
-    ∀ p q, pop p q bufs = None.
-
   Lemma bufs_empty_delete {A} (bufs : bufsT participant participant A) p :
     bufs_empty bufs -> bufs_empty (delete p bufs).
   Proof.
@@ -260,41 +257,6 @@ End pushpop.
 
 Section bufs_typed.
 
-  Inductive rglobal_type : Type :=
-    | MessageR n : option (fin n) -> participant -> participant ->
-                  (fin n -> type) -> (fin n -> rglobal_type) -> rglobal_type
-    | ContinueR : global_type -> rglobal_type.
-
-  Inductive rproj (r : participant) : rglobal_type -> session_type -> Prop :=
-    | rproj_send n q ts Gs σs :
-        q ≠ r -> (∀ i, rproj r (Gs i) (σs i)) ->
-          rproj r (MessageR n None r q ts Gs) (SendT n q ts σs)
-    | rproj_recv n o p ts Gs σs :
-        p ≠ r -> (∀ i, rproj r (Gs i) (σs i)) ->
-          rproj r (MessageR n o p r ts Gs) (RecvT n p ts σs)
-    | rproj_skip n p q ts Gs σ :
-        p ≠ r -> q ≠ r -> (∀ i, rproj r (Gs i) σ) ->
-          rproj r (MessageR (S n) None p q ts Gs) σ
-    | rproj_buf_skip n i p q ts Gs σ :
-        q ≠ r -> rproj r (Gs i) σ ->
-          rproj r (MessageR n (Some i) p q ts Gs) σ
-    | rproj_continue G σ :
-        proj r G σ -> rproj r (ContinueR G) σ.
-
-
-
-  Inductive sbufprojs : rglobal_type -> sbufsT -> Prop :=
-    | bp_skip n p q ts Gs bufs :
-        pop p q bufs = None -> (∀ i, sbufprojs (Gs i) bufs) ->
-        sbufprojs (MessageR n None p q ts Gs) bufs
-    | bp_here n p q i bufs bufs' ts Gs :
-        pop p q bufs = Some ((fin_to_nat i, ts i), bufs') ->
-        sbufprojs (Gs i) bufs' ->
-        sbufprojs (MessageR n (Some i) p q ts Gs) bufs
-    | bp_end G' bufs : bufs_empty bufs -> sbufprojs (ContinueR G') bufs.
-
-
-
   Lemma sbufs_typed_pop' (σs : gmap participant session_type)
     (bufs bufs' : bufsT participant participant sentryT)
     (n : nat) (p q : participant) t i ts ss :
@@ -313,240 +275,6 @@ Section bufs_typed.
     constructor; sdec. intros ?[]. smap.
   Qed.
 
-  Inductive pushUG (p q : participant) (n : nat) (i : fin n) : type -> global_type -> rglobal_type -> Prop :=
-    | pushU_skip n' p' q' t ts Gs Gs' :
-        p' ≠ p -> (∀ j, pushUG p q n i t (Gs j) (Gs' j)) ->
-        pushUG p q n i t (Message (S n') p' q' ts Gs) (MessageR (S n') None p' q' ts Gs')
-    | pushU_here ts Gs :
-        pushUG p q n i (ts i) (Message n p q ts Gs) (MessageR n (Some i) p q ts (λ j, ContinueR (Gs j))).
-
-  Inductive pushG (p q : participant) (n : nat) (i : fin n) : type -> rglobal_type -> rglobal_type -> Prop :=
-    | push_skipN n' p' q' ts Gs Gs' t :
-        p' ≠ p -> (∀ j, pushG p q n i t (Gs j) (Gs' j)) ->
-        pushG p q n i t (MessageR (S n') None p' q' ts Gs) (MessageR (S n') None p' q' ts Gs')
-    | push_skipS n' i' p' q' ts Gs Gs' t :
-        pushG p q n i t (Gs i') (Gs' i') -> (∀ j, j ≠ i' -> Gs j = Gs' j) ->
-        pushG p q n i t (MessageR n' (Some i') p' q' ts Gs) (MessageR n' (Some i') p' q' ts Gs')
-    | push_here ts Gs :
-        pushG p q n i (ts i) (MessageR n None p q ts Gs) (MessageR n (Some i) p q ts Gs)
-    | push_cont G G' t : pushUG p q n i t G G' -> pushG p q n i t (ContinueR G) G'.
-
-  Ltac inv H := inversion H; simplify_eq; clear H.
-
-  Lemma send_pushUG p q G n ts σs i :
-    proj p G (SendT n q ts σs) -> ∃ G', pushUG p q n i (ts i) G G'.
-  Proof.
-    intros H.
-    inv H; eauto using pushUG.
-    assert (∀ j, ∃ G', pushUG p q n i (ts i) (G0 j) G').
-    {
-      intros j.
-      specialize (H2 j).
-      specialize (H3 j).
-      revert H2 H3.
-      generalize (G0 j). clear. intros G Hproj Hoc.
-      induction Hoc; inv Hproj; eauto using pushUG.
-      assert (∀ i0, ∃ G' : rglobal_type, pushUG p q n i (ts i) (g i0) G').
-      { eauto. }
-      apply fin_choice in H1 as [].
-      eauto using pushUG.
-    }
-    eapply fin_choice in H as []; eauto using pushUG.
-  Qed.
-
-  Lemma send_pushG p q G n ts σs i :
-    rproj p G (SendT n q ts σs) -> ∃ G', pushG p q n i (ts i) G G'.
-  Proof.
-    intros H.
-    induction G; inv H; eauto using pushG.
-    - assert (∀ j, ∃ G', pushG p q n i (ts i) (r j) G') as Hc; eauto.
-      apply fin_choice in Hc as [Gs' HGs'].
-      eexists. constructor; eauto.
-    - edestruct H0; eauto.
-      eexists (MessageR _ _ _ _ _ (λ j, if decide (j = i1) then x else r j)).
-      econstructor; last intros; case_decide; simplify_eq; eauto.
-    - edestruct send_pushUG; eauto using pushG.
-  Qed.
-
-  Lemma pushUG_send p q n i G G' t ts σs :
-    pushUG p q n i t G G' -> proj p G (SendT n q ts σs) -> rproj p G' (σs i).
-  Proof.
-    induction 1; intros Hproj; inv Hproj; eauto using rproj.
-  Qed.
-
-  Lemma pushG_send p q n i G G' t ts σs :
-    pushG p q n i t G G' -> rproj p G (SendT n q ts σs) -> rproj p G' (σs i).
-  Proof.
-    induction 1; intros Hproj; inv Hproj; eauto using rproj, pushUG_send.
-  Qed.
-
-  Lemma pushUG_other p q r n i G G' σ t :
-    r ≠ p -> pushUG p q n i t G G' -> proj r G σ -> rproj r G' σ.
-  Proof.
-    intros Hneq Hpush. revert σ; induction Hpush; intros σ Hproj;
-    inv Hproj; eauto using rproj.
-    - constructor.
-      + intros ->. apply H2. eauto using occurs_in.
-      + intros ->. apply H2. eauto using occurs_in.
-      + intro. eapply H1. constructor. intros Q.
-        eapply H2. eauto using occurs_in.
-    - econstructor; eauto.
-      { intros ->. apply H; eauto using occurs_in. }
-      econstructor. constructor. intros Q.
-      apply H. econstructor. eauto using occurs_in.
-  Qed.
-
-  Lemma pushG_other p q r n i G G' σ t :
-    r ≠ p -> pushG p q n i t G G' -> rproj r G σ -> rproj r G' σ.
-  Proof.
-    intros Hneq Hpush. revert σ; induction Hpush; intros σ Hproj;
-    inv Hproj; eauto using rproj, pushUG_other.
-    econstructor; eauto. intros j.
-    destruct (decide (j = i')); subst; eauto.
-    rewrite -H; eauto.
-  Qed.
-
-  Lemma proj_consistent p q n i t G G' :
-    pushG p q n i t G G' -> ¬ rproj q G EndT.
-  Proof.
-    induction 1; intros Hproj; inv Hproj.
-    - eapply H1. eauto. Unshelve. exact 0%fin.
-    - induction H; inv H1; eauto using occurs_in.
-      eapply H2. econstructor. intro.
-      eauto using occurs_in. Unshelve. exact 0%fin. exact 0%fin.
-  Qed.
-
-  Lemma pushUG_bufs p q n i t G G' bufs :
-    pushUG p q n i t G G' -> bufs_empty bufs -> is_present p q bufs ->
-    sbufprojs G' (push p q (fin_to_nat i,t) bufs).
-  Proof.
-    induction 1; eauto using pop_push_None, pop_push_single, sbufprojs.
-  Qed.
-
-  Lemma pushG_bufs p q n i G G' bufs t :
-    pushG p q n i t G G' -> is_present p q bufs ->
-    sbufprojs G bufs ->
-    sbufprojs G' (push p q (fin_to_nat i,t) bufs).
-  Proof.
-    intros Hpush. revert bufs. induction Hpush; intros bufs Hpres Hsb; inv Hsb;
-    eauto using sbufprojs, pushUG_bufs, pop_push_single, pop_is_present, pop_push_Some, pop_push_None.
-  Qed.
-
-  (* Lemma sbufs_typed_push (bufss : bufsT participant participant sentryT)
-                        (σs : gmap participant session_type)
-                        (n : nat) (i : fin n) (p q : participant) ts ss :
-    σs !! p = Some (SendT n q ts ss) ->
-    sbufs_typed bufss σs ->
-    sbufs_typed (push p q (fin_to_nat i,ts i) bufss) (<[p:=ss i]> σs).
-  Proof.
-  Admitted. *)
-    (* intros Hp [Hdb [G [Hprojs Hsb]]].
-    split. { rewrite dom_insert_lookup_L; eauto.
-             apply dom_valid_push; eauto. apply elem_of_dom; eauto. }
-    pose proof (Hprojs p) as Hproj. rewrite Hp in Hproj. simpl in *.
-    edestruct send_pushG as [G' H]; first done.
-    exists G'. split.
-    - intros r. rewrite lookup_insert_spec.
-      case_decide; subst; simpl; last eauto using pushG_other.
-      eapply pushG_send; eauto.
-    - eapply pushG_bufs; eauto.
-      eapply dom_valid_is_present; eauto; apply elem_of_dom.
-      + rewrite ?Hp; eauto.
-      + specialize (Hprojs q).
-        destruct (σs !! q); eauto.
-        simpl in *. exfalso. eapply proj_consistent; eauto.
-  Qed. *)
-
-  Inductive popG (p q : participant) (n : nat) (i : fin n) : type -> rglobal_type -> rglobal_type -> Prop :=
-    | pop_skipN n' p' q' ts Gs Gs' t :
-        q' ≠ q -> (∀ j, popG p q n i t (Gs j) (Gs' j)) ->
-        popG p q n i t (MessageR (S n') None p' q' ts Gs) (MessageR (S n') None p' q' ts Gs')
-    | pop_skipS n' i' p' q' ts Gs Gs' t :
-        q' ≠ q -> popG p q n i t (Gs i') (Gs' i') -> (∀ j, j ≠ i' -> Gs j = Gs' j) ->
-        popG p q n i t (MessageR n' (Some i') p' q' ts Gs) (MessageR n' (Some i') p' q' ts Gs')
-    | pop_here ts Gs :
-        popG p q n i (ts i) (MessageR n (Some i) p q ts Gs) (Gs i).
-
-  Lemma sbufprojs_popG (G : rglobal_type)
-    (bufs bufs' : bufsT participant participant sentryT)
-    (n : nat) (p q : participant) t i ts ss :
-    rproj q G (RecvT n p ts ss) ->
-    pop p q bufs = Some((i,t),bufs') ->
-    sbufprojs G bufs -> ∃ G' i', i = fin_to_nat i' ∧ popG p q n i' (ts i') G G'.
-  Proof.
-    intros Hp. revert bufs bufs'. induction G; intros bufs bufs' Hpop Hsb; inv Hsb.
-    - inv Hp.
-      assert (∀ j, ∃ G' i', i = fin_to_nat i' ∧ popG p q n i' (ts i') (r j) G') as Q.
-      { intros. edestruct H; eauto. }
-      apply fin_choice in Q as [Gs' HG].
-      destruct (HG 0%fin) as [j []]. subst.
-      eexists _,_; split; eauto.
-      econstructor; eauto. intros. edestruct HG as [? []].
-      simplify_eq. eauto.
-    - inv Hp.
-      + eexists _,_. rewrite Hpop in H7. simplify_eq.
-        split; eauto using pop_here.
-      + assert (∃ bufs'', pop p q bufs'0 = Some (i, t, bufs'')) as []; eauto using pop_swap'.
-        edestruct H as [G' [i' [-> HG]]]; eauto.
-        eexists (MessageR _ _ _ _ _ (λ i, if decide (i = i1) then G' else r i)),_.
-        split; eauto. econstructor; eauto. sdec. intros. sdec.
-    - rewrite H0 in Hpop. sdec.
-  Qed.
-
-  Lemma popG_recv p q n i G G' t ts σs :
-    popG p q n i t G G' -> rproj q G (RecvT n p ts σs) -> rproj q G' (σs i).
-  Proof.
-    induction 1; intros Hproj; inv Hproj; eauto using rproj.
-  Qed.
-
-  Lemma popG_other p q r n i G G' σ t :
-    r ≠ q -> popG p q n i t G G' -> rproj r G σ -> rproj r G' σ.
-  Proof.
-    intros Hneq Hpush. revert σ; induction Hpush; intros σ Hproj;
-    inv Hproj; eauto using rproj.
-    econstructor; eauto.
-    intros j. destruct (decide (j = i')); sdec.
-    rewrite -H0; eauto.
-  Qed.
-
-  Lemma popG_sbufprojs p q n bufs bufs' t t' i G G' :
-    popG p q n i t G G' ->
-    pop p q bufs = Some (fin_to_nat i, t', bufs') ->
-    sbufprojs G bufs -> t = t' ∧ sbufprojs G' bufs'.
-  Proof.
-    intros HpopG. revert bufs bufs'. induction HpopG; simpl; intros bufs bufs' Hpop Hsb;
-    inv Hsb; eauto using sbufprojs.
-    - edestruct H1; eauto. clear H3. subst.
-      split; eauto.
-      econstructor; eauto using pop_pop_None.
-      intros. edestruct H1; eauto.
-    - assert (∃ bufs'' : sbufsT, pop p q bufs'0 = Some (fin_to_nat i,t', bufs'')) as []
-        by eauto using pop_swap'.
-      edestruct IHHpopG; [|eauto|]; eauto. subst.
-      split; eauto. econstructor; eauto using pop_commute.
-      Unshelve. exact 0%fin.
-  Qed.
-
-  (* Lemma sbufs_typed_pop (σs : gmap participant session_type)
-    (bufs bufs' : bufsT participant participant sentryT)
-    (n : nat) (p q : participant) t i ts ss :
-    σs !! q = Some (RecvT n p ts ss) ->
-    pop p q bufs = Some((i,t),bufs') ->
-    sbufs_typed bufs σs -> ∃ i', i = fin_to_nat i' ∧ t = ts i' ∧
-      sbufs_typed bufs' (<[ q := ss i' ]> σs).
-  Proof.
-  Admitted. *)
-    (* intros Hp Hpop [Hdv [G [Hprojs Hsb]]].
-    pose proof (Hprojs q) as Hproj. rewrite Hp in Hproj. simpl in *.
-    edestruct sbufprojs_popG as (G' & i' & Q & HpopG); eauto. subst.
-    eexists; split; eauto.
-    edestruct popG_sbufprojs; eauto. subst.
-    split; eauto.
-    split. { rewrite dom_insert_lookup_L; eauto. eapply dom_valid_pop; eauto. }
-    exists G'. split; eauto.
-    intros r. smap; eauto using popG_other, popG_recv.
-  Qed. *)
-
   Definition entries_typed (bufs : bufsT participant participant entryT)
                            (sbufs : bufsT participant participant sentryT) : rProp :=
     [∗ map] p ↦ bfs;sbfs ∈ bufs;sbufs,
@@ -558,11 +286,6 @@ Section bufs_typed.
     ∃ sbufs, ⌜⌜ sbufs_typed sbufs σs ⌝⌝ ∗ entries_typed bufs sbufs.
 
   Global Instance bufs_typed_params : Params bufs_typed 1 := {}.
-
-  Global Instance rproj_Proper p G : Proper ((≡) ==> (≡)) (rproj p G).
-  Proof.
-    intros ???. apply session_type_extensionality in H. subst. done.
-  Qed.
 
   Global Instance session_typed_leibniz : LeibnizEquiv session_type.
   Proof.
@@ -576,25 +299,6 @@ Section bufs_typed.
 
   Global Instance bufs_typed_Proper bufs : Proper ((≡) ==> (≡)) (bufs_typed bufs).
   Proof. solve_proper. Qed.
-
-  (* Lemma sbufs_Some_present σs p q n ts ss sbufs (i : fin n) :
-    σs !! p = Some (SendT n q ts ss) ->
-    sbufs_typed sbufs σs ->
-    is_present p q sbufs.
-  Proof.
-  Admitted. *)
-    (* intros Hp [Hdv [G [Hprojs bufs]]].
-    pose proof (Hprojs p) as Hproj.
-    rewrite Hp in Hproj. simpl in *.
-    eapply send_pushG in Hproj as [G' HpushG]. Unshelve. 2: eauto.
-    assert (¬ rproj q G EndT); eauto using proj_consistent.
-    destruct (σs !! q) eqn:E.
-    {
-      eapply dom_valid_is_present; eauto; apply elem_of_dom; rewrite ?E ?Hp; eauto.
-    }
-    specialize (Hprojs q).
-    rewrite E in Hprojs. done.
-  Qed. *)
 
   Definition same_structure (bufs : bufsT participant participant entryT) (sbufs : bufsT participant participant sentryT) :=
     ∀ p, match bufs !! p, sbufs !! p with
@@ -659,24 +363,6 @@ Section bufs_typed.
       assert (p ∉ dom bufs). { apply not_elem_of_dom. done. }
       rewrite -Q in H. set_solver.
   Qed.
-(*
-  Definition only_changes {A} p q (bufs bufs' : bufsT participant participant A) :=
-    ∀ r, match bufs !! r, bufs' !! r with
-         | Some bfs,Some bfs' =>
-           ∀ s, match bfs !! s, bfs' !! s with
-                | Some buf, Some buf' => p ≠ s -> q ≠ r -> buf = buf'
-                | None, None => True
-                | _,_ => False
-                end
-         | None,None => True
-         | _,_ => False
-         end.
-
-  Lemma only_changes_entries_typed p q bufs bufs' sbufs sbufs' :
-    only_changes p q bufs bufs' ->
-    only_changes p q sbufs sbufs' ->
-    entries_typed bufs sbufs -∗
-    entries_typed sbufs sbufs' *)
 
   Lemma push_is_Some `{Countable A, Countable B} {V} p q r x (bufs : bufsT A B V) :
     is_Some (bufs !! r) -> is_Some (push p q x bufs !! r).
@@ -852,23 +538,6 @@ Section bufs_typed.
     iExists _. iSplit; first done. iFrame.
   Qed.
 
-  (* Lemma sbufs_typed_dealloc sbufs σs p :
-    σs !! p = Some EndT ->
-    sbufs_typed sbufs σs ->
-    sbufs_typed (delete p sbufs) (delete p σs).
-  Proof.
-  Admitted. *)
-    (* intros Hp [Hdv [G [Hprojs Hsbufs]]].
-    split. { rewrite dom_delete_L. eapply dom_valid_delete; done. }
-    exists G.
-    assert (rproj p G EndT) as Hprojp.
-    { specialize (Hprojs p). rewrite Hp in Hprojs. done. }
-    split. {intros p'. rewrite lookup_delete_spec. case_decide; subst; eauto. }
-    clear Hp Hdv Hprojs σs.
-    revert sbufs Hsbufs. induction G; intros; inv Hprojp; inv Hsbufs;
-    eauto using sbufprojs,pop_delete_None,pop_delete_Some,bufs_empty_delete.
-  Qed. *)
-
 
   Lemma entries_typed_delete p bufs sbufs :
     buf_empty sbufs p ->
@@ -924,19 +593,6 @@ Section bufs_typed.
     destruct l eqn:E''; smap.
   Qed.
 
-  (* Lemma sbufs_typed_end_empty σs p bufs :
-    σs !! p = Some EndT ->
-    sbufs_typed bufs σs ->
-    buf_empty bufs p.
-  Proof.
-  Admitted. *)
-    (* intros Hp [Hdv [G [Hprojs Hsb]]].
-    specialize (Hprojs p).
-    rewrite Hp in Hprojs. simpl in *.
-    clear Hdv.
-    induction Hsb; inv Hprojs; eauto using bufs_empty_buf_empty,buf_empty_pop.
-    Unshelve. exact 0%fin.
-  Qed. *)
 
   Lemma bufs_typed_dealloc bufss σs p :
     σs !! p ≡ Some EndT ->
@@ -952,16 +608,6 @@ Section bufs_typed.
     iSplit. { iPureIntro. apply sbufs_typed_dealloc; done. }
     iApply entries_typed_delete; eauto using sbufs_typed_end_empty.
   Qed.
-
-  (* Lemma sbufs_typed_empty : sbufs_typed ∅ ∅.
-  Proof.
-  Admitted. *)
-    (* split. { rewrite dom_empty_L. apply dom_valid_empty. }
-    exists (ContinueR EndG). split.
-    - intros p. rewrite lookup_empty /=.
-      constructor. constructor. intros H. inversion H.
-    - econstructor. intros ??. unfold pop. rewrite lookup_empty //.
-  Qed. *)
 
   Lemma entries_typed_empty : emp ⊣⊢ entries_typed ∅ ∅.
   Proof.
@@ -993,15 +639,6 @@ Section bufs_typed.
     iDestruct (big_sepM2_empty_l with "H") as %->.
     rewrite <-entries_typed_empty. done.
   Qed.
-
-  (* Lemma sbufs_typed_empty_inv σs :
-    sbufs_typed ∅ σs -> σs = ∅.
-  Proof.
-  Admitted. *)
-    (* intros [Hdv [G [Hprojs Hsbufs]]].
-    apply dom_valid_empty_inv in Hdv.
-    apply dom_empty_iff_L in Hdv. done.
-  Qed. *)
 
   Lemma bufs_typed_empty_inv σs :
     bufs_typed ∅ σs ⊢ ⌜⌜ σs = ∅ ⌝⌝.
@@ -1054,18 +691,6 @@ Section bufs_typed.
     consistent n σs ->
     sbufs_typed (init_chans n) (fin_gmap n σs).
   Proof. done. Qed.
-  (* destruct Hcons as [G [Hprojs1 Hprojs2]].
-      split; first by eauto using dom_valid_init, fin_gmap_dom.
-      exists (ContinueR G).
-      split.
-      - intros p.
-        destruct (decide (p < n)).
-        + rewrite -(fin_to_nat_to_fin _ _ l).
-          rewrite fin_gmap_lookup. simpl.
-          eauto using rproj.
-        + rewrite fin_gmap_lookup_ne; last lia.
-          simpl. eauto using rproj with lia.
-      - econstructor. eapply bufs_empty_init_chans. *)
 
   Lemma bufs_typed_init n σs :
     consistent n σs ->
@@ -1117,16 +742,6 @@ Section bufs_typed.
     intros []. sdec.
   Qed.
 
-  (* Lemma sbufs_typed_recv bufss σs p :
-    is_Some (σs !! p) ->
-    sbufs_typed bufss σs -> is_Some (bufss !! p).
-  Proof.
-  Admitted. *)
-    (* intros Hp [Hdv [G [Hprojs Hsbufs]]].
-    eapply dom_valid_same_dom; eauto.
-    apply elem_of_dom. done.
-  Qed. *)
-
   Lemma entries_typed_same_dom bufs sbufs :
     entries_typed bufs sbufs ⊢ ⌜ dom bufs = dom sbufs ⌝.
   Proof.
@@ -1146,56 +761,6 @@ Section bufs_typed.
     apply elem_of_dom. rewrite Hdom.
     apply elem_of_dom. done.
   Qed.
-
-
-  (* Lemma sbufs_typed_progress bufss σs :
-    sbufs_typed bufss σs -> bufss = ∅ ∨ can_progress bufss σs.
-  Proof.
-  Admitted. *)
-    (* intros [Hdv [G [Hprojs Hsbufs]]].
-    inv Hsbufs.
-    - right.
-      unfold can_progress.
-      specialize (Hprojs p).
-      exists p.
-      destruct (σs !! p); last (inversion Hprojs; simplify_eq).
-      eexists _; split; first done.
-      destruct s; eauto. simpl in *.
-      inversion Hprojs; simplify_eq.
-    - right.
-      specialize (Hprojs q).
-      unfold can_progress.
-      exists q.
-      destruct (σs !! q); last (inversion Hprojs; simplify_eq). simpl in *.
-      exists s. split; eauto.
-      destruct s; eauto.
-      inv Hprojs; eauto.
-  - destruct (classic (bufss = ∅)) as [|Q]; eauto.
-    eapply map_choose in Q as [p [x Hp]].
-    right. unfold can_progress.
-    destruct G'.
-    + specialize (Hprojs p0).
-      exists p0.
-      destruct (σs !! p0); simpl in *.
-      * inversion Hprojs; subst.
-        remember (Message n p0 p1 t g).
-        inversion H1; simplify_eq.
-        { eexists. split; eauto. simpl. eauto. }
-        exfalso. eauto using occurs_in.
-      * inversion Hprojs; simplify_eq. inversion H1; simplify_eq.
-        exfalso. eauto using occurs_in.
-    + specialize (Hprojs p).
-      exists p.
-      destruct (σs !! p) eqn:E; last first.
-      { apply not_elem_of_dom in E.
-        exfalso. apply E.
-        eapply dom_valid_same_dom; eauto. }
-      eexists. split; first done.
-      destruct s; eauto.
-      simpl in *.
-      inversion Hprojs; simplify_eq.
-      inversion H1; simplify_eq.
-  Qed. *)
 
   Lemma entries_typed_can_progress bufs sbufs σs :
     can_progress sbufs σs ->
